{
 "cells": [
  {
   "cell_type": "markdown",
   "metadata": {},
   "source": [
    "# Problem 1 [40 points] Lyapunov stability for a non-autonomous nonlinear system\n",
    "\n",
    "Consider the continuous-time non-autonomous system\n",
    "\n",
    "$$\\begin{align*}\n",
    "\\dot{x}_{1} &= -x_{1} - g(t)x_{2},\\\\\n",
    "\\dot{x}_{2} &= x_{1} - x_{2},\n",
    "\\end{align*}\n",
    "$$\n",
    "\n",
    "where the state vector $(x_1,x_2)^{\\top}\\in\\mathbb{R}^{2}$. The function $g(t)$ is $C^{1}$ in time $t$, satisfies $0 \\leq g(t) \\leq k$ for some constant $k$, and $\\dot{g}(t) \\leq g(t)$ for all $t\\geq 0$."
   ]
  },
  {
   "cell_type": "markdown",
   "metadata": {},
   "source": [
    "## (a) [10 points] Fixed point\n",
    "\n",
    "**Prove that** the origin $(0,0)^{\\top}$ is a fixed point. \n",
    "\n",
    "1.\n",
    "$$\\begin{align*}\n",
    "&\\forall t \\geq 0,\\\\\n",
    "\\dot{x}_{1} &= -0 - g(t) * 0 &= 0,\\\\\n",
    "\\dot{x}_{2} &= 0 - 0 &= 0,\n",
    "\\end{align*}\n",
    "$$\n",
    "\n",
    "Thus by definition $(0,0)^{\\top}$ is a fixed point"
   ]
  },
  {
   "cell_type": "markdown",
   "metadata": {},
   "source": [
    "## (b) [30 points] Origin is GES\n",
    "\n",
    "Use the Lyapunov function $V(t,x_1,x_2) := x_1^2 + (1 + g(t))x_2^2$ to **prove that** the origin is globally exponentially stable (GES).\n",
    "\n",
    "(**Hint:** Lec. 5, p. 3).\n",
    "\n",
    "1.\n",
    "\\begin{align*}\n",
    "0 \\leq x_{2}^{2} \\leq x_{2}^{2} + x_{1}^{2}\\\\\n",
    "0 \\leq x_{2}^{2} \\leq \\lVert x \\rVert^{2}\\\\\n",
    "0 \\leq g(t) x_{2}^{2} \\leq k \\lVert x \\rVert^{2}\\\\\n",
    "\\lVert x \\rVert^{2} \\leq g(t) x_{2}^{2} + \\lVert x \\rVert^{2} \\leq (1+k) \\lVert x \\rVert^{2}\\\\\n",
    "\\lVert x \\rVert^{2} \\leq g(t) x_{2}^{2} + x_{2}^{2} + x_{1}^{2} \\leq (1+k) \\lVert x \\rVert^{2}\\\\\n",
    "\\lVert x \\rVert^{2} \\leq (g(t) + 1) x_{2}^{2} + x_{1}^{2} \\leq (1+k) \\lVert x \\rVert^{2}\\\\\n",
    "\\lVert x \\rVert^{2} \\leq V(t, x_{1}, x_{2}) \\leq (1+k) \\lVert x \\rVert^{2}\\\\\n",
    "\\end{align*}\n",
    "<br>\n",
    "2. We take 1. above $k_{1} = 1, k_{2} = (1 + k), \\alpha = 2$:\n",
    "\\begin{align*}\n",
    "k_{1} \\lVert x \\rVert^{\\alpha} \\leq V(t, x_{1}, x_{2}) \\leq k_{2} \\lVert x \\rVert^{\\alpha}\n",
    "\\end{align*}\n",
    "<br>\n",
    "3. \n",
    "\\begin{align}\n",
    "\\frac{\\partial{V}}{\\partial{t}} & = 0 + 0 + \\frac{\\partial{}}{\\partial{t}} g(t)x_{2}^{2}\\\\\n",
    "& = x_{2}^{2}\\dot{g}(t)\n",
    "\\end{align}\n",
    "<br>\n",
    "4.\n",
    "\\begin{align}\n",
    "\\frac{\\partial{V}}{\\partial{x}} & = \\begin{bmatrix} \\frac{\\partial{V}}{\\partial{x_{1}}} \\\\ \\frac{\\partial{V}}{\\partial{x_{2}}} \\end{bmatrix}\\\\\n",
    "& = \\begin{bmatrix} 2x_{1} \\\\ 2x_{2}(1+g) \\end{bmatrix}\\\\\n",
    "\\end{align}\n",
    "<br>\n",
    "5. Combining 3. 4. above:\n",
    "\\begin{align}\n",
    "\\dot{V} & = \\frac{\\partial{V}}{\\partial{t}} + \\frac{\\partial{V}}{\\partial{x}} f(t, x_{1}, x_{2})\\\\\n",
    "& = x_{2}^{2}\\dot{g}(t) + 2x_{1}(-x_1 - gx_2) + (x_1 - x_2)(2x_2)(1+g)\\\\\n",
    "& = -2x_1^{2} + 2x_1x_2 + x_2^{2}(\\dot{g} -2 - 2g)\\\\\n",
    "\\end{align}\n",
    "<br>\n",
    "6. Since  $\\dot{g} \\leq g$:\n",
    "\\begin{align}\n",
    "\\dot{g} - 2 - 2g \\leq g - 2 - 2g = -2 - g\\\\\n",
    "\\end{align}\n",
    "and further $-2 - g \\leq -2$:\n",
    "\\begin{align}\n",
    "0 \\leq g \\leq k\\\\\n",
    "-k \\leq -g \\leq 0\\\\\n",
    "-2-k \\leq -2-g \\leq -2\\\\\n",
    "\\end{align}\n",
    "therefore $\\dot{g} - 2 - 2g \\leq -2$\n",
    "<br>\n",
    "7. Combinining 5. and 6. above: $\\dot{V} \\leq  2x_1x_2 - 2x_1^{2} - 2x_2^{2}$\n",
    "<br>\n",
    "8. $(x_1 - x_2)^{2}$ is non-negative, so:\n",
    "\\begin{align}\n",
    "\\dot{V} & \\leq  2x_1x_2 - 2x_1^{2} - 2x_2^{2}\\\\\n",
    "& \\leq 2x_1x_2 - 2x_1^{2} - 2x_2^{2} + (x_1 - x_2)^{2}\\\\\n",
    "& = 2x_1x_2 - 2x_1^{2} - 2x_2^{2} + x_1^{2} - 2x_1x_2 + x_2^{2}\\\\\n",
    "& = - 2x_1^{2} - 2x_2^{2} + x_1^{2} + x_2^{2}\\\\\n",
    "& = - x_1^{2} - x_2^{2}\\\\\n",
    "& = -1 (x_1^{2} + x_2^{2})\\\\\n",
    "& = -1 \\lVert x \\rVert^{2}\\\\\n",
    "& \\leq k_{3} \\lVert x \\rVert^{\\alpha}, k_{3} = 1, \\alpha = 2\\\\\n",
    "\\end{align}\n",
    "<br>\n",
    "9. So from  8. and 2. since they hold true $\\forall x \\in {R^{n}}$ and by Lec 5 pg. 3, the origin **is GES**."
   ]
  },
  {
   "cell_type": "markdown",
   "metadata": {},
   "source": [
    "# Problem 2 [60 points] Lyapunov stability for a rotating rigid spacecraft\n",
    "\n",
    "The controlled dynamics for a rotating rigid spacecraft is given by the Euler equation\n",
    "\n",
    "\\begin{align*}\n",
    "J_{1}\\dot{\\omega}_{1} = \\left(J_{2} - J_{3}\\right)\\omega_{2}\\omega_{3} + \\tau_{1},\\\\\n",
    "    J_{2}\\dot{\\omega}_{2} = \\left(J_{3} - J_{1}\\right)\\omega_{3}\\omega_{1} + \\tau_{2},\\\\\n",
    "    J_{3}\\dot{\\omega}_{3} = \\left(J_{1} - J_{2}\\right)\\omega_{1}\\omega_{2} + \\tau_{3},\n",
    "\\end{align*}\n",
    "where the parameters $J_1,J_2,J_3>0$ denote the principal moments of inertia; the state vector $(\\omega_1,\\omega_2,\\omega_3)^{\\top}\\in\\mathbb{R}^{3}$ denotes the spacecraftâ€™s angular velocity (in rad/s) along its principal axes; and the control vector $(\\tau_1,\\tau_2,\\tau_3)^{\\top}$ denotes the torque input applied about the principal axes."
   ]
  },
  {
   "cell_type": "markdown",
   "metadata": {},
   "source": [
    "## (a) [2 + (2 + 6) = 10 points] Fixed points in the absence of control\n",
    "\n",
    "Suppose that the controls $\\tau_1 = \\tau_2 = \\tau_3 \\equiv 0$.\n",
    "\n",
    "(i) **Argue that** origin is a fixed point.\n",
    "\n",
    "1. when $(\\omega_{1}, \\omega_{2}, \\omega_{3})^{T} = 0$\n",
    "\n",
    "\\begin{align*}\n",
    "J_{1}\\dot{\\omega}_{1} = \\left(J_{2} - J_{3}\\right)0+ 0 \\rightarrow J_{1}\\dot{\\omega}_{1} = 0 \\rightarrow \\dot{\\omega}_{1} = 0,\\\\\n",
    "J_{2}\\dot{\\omega}_{2} = \\left(J_{3} - J_{1}\\right)0 + 0 \\rightarrow J_{2}\\dot{\\omega}_{2} = 0 \\rightarrow \\dot{\\omega}_{2} = 0,\\\\\n",
    "J_{3}\\dot{\\omega}_{3} = \\left(J_{1} - J_{2}\\right)0 + 0 \\rightarrow J_{3}\\dot{\\omega}_{3} = 0 \\rightarrow \\dot{\\omega}_{3} = 0,\n",
    "\\end{align*}\n",
    "\n",
    "(ii) **How many fixed points other than origin** are there? **Explain what physical motions** do these non-origin fixed points correspnd to?\n",
    "\n",
    "1. All 3 equations above include 2 / 3 state terms. So for any states where 2 of the 3 dimensions of $\\omega_{i} = 0$, all 3 equations will yield 0. i.e. $(\\omega_{1}, 0, 0)^{T}, (0, \\omega_{2}, 0)^{T}, (0, 0, \\omega_{3})^{T}$\n",
    "\n",
    "2. For the nonzero elements of those 3 state vectors, it doest *not* matter what the nonzero element is, so there is an *infinite* # of points other than the origin.\n",
    "\n",
    "3. The physical meaning of those 3 state vectors is when the spacecraft is rotating about *1* of the principal axes while stationary about the other axes. In these states, the spacecraft dynamics do *not* change, the spacecraft will continue rotating about that axis at the same angular velocity indefinitely."
   ]
  },
  {
   "cell_type": "markdown",
   "metadata": {},
   "source": [
    "## (b) [(10 + 5) + 10 = 25] S/AS in the absence of control\n",
    "\n",
    "As in part (a), assume that the controls $\\tau_1 = \\tau_2 = \\tau_3 \\equiv 0$.\n",
    "\n",
    "(i) By constructing a suitable Lyapunov function, **prove that** the origin is stable (S). From this analysis, **what can you conclude** about the asymptotic stability (AS) of the origin?\n",
    "\n",
    "1. Let $V = \\frac{1}{2}\\begin{bmatrix} \\omega_{1} & \\omega_{2} & \\omega_{3} \\end{bmatrix} \\begin{bmatrix} J_{1} & 0 & 0 \\\\ 0 & J_{2} & 0 \\\\ 0 & 0 & J_{3} \\end{bmatrix} \\begin{bmatrix} \\omega_{1} \\\\ \\omega_{2} \\\\ \\omega_{3} \\end{bmatrix} = \\frac{1}{2}(J_{1}\\omega_{1}^{2} + J_{2}\\omega_{2}^{2} + J_{3}\\omega_{3}^{2})$ where $P = \\begin{bmatrix} J_{1} & 0 & 0 \\\\ 0 & J_{2} & 0 \\\\ 0 & 0 & J_{3} \\end{bmatrix}$\n",
    "<br>\n",
    "2. Knowing $J_{1}, J_{2}, J_{3} > 0$, $V = \\frac{1}{2}(J_{1}\\omega_{1}^{2} + J_{2}\\omega_{2}^{2} + J_{3}\\omega_{3}^{2}) > 0$ $\\forall \\begin{bmatrix} \\omega_{1} & \\omega_{2} & \\omega_{3} \\end{bmatrix} \\rightarrow$ P is positive definite matrix.\n",
    "<br>\n",
    "3. We can show that $\\dot{V}$ is negative **semi-definite**:\n",
    "\\begin{align}\n",
    "& \\dot{V} = \\omega_{1}(J_{1}*\\dot\\omega_{1}) + \\omega_{2}(J_{2}*\\dot\\omega_{2}) + \\omega_{3}(J_{3}*\\dot\\omega_{3}) \\\\\n",
    "& = \\omega_{1}(J_{2}-J_{3})\\omega_{2}\\omega_{3} + \\omega_{2}(J_{3}-J_{1})\\omega_{1}\\omega_{3} + \\omega_{3}(J_{1}-J_{2})\\omega_{1}\\omega_{1} \\\\\n",
    "& = \\omega_{1}\\omega_{2}\\omega_{3}(J_{2}-J_{3} + J_{3}-J_{1} + J_{1}-J_{2})\\\\\n",
    "& = \\omega_{1}\\omega_{2}\\omega_{3}(J_{2}-J_{3} + J_{3}-J_{1} + J_{1}-J_{2})\\\\\n",
    "& = 0\\\\\n",
    "\\end{align}\n",
    "<br>\n",
    "4. Therefore, from 2. and 3. above, and by Lec 3. pg 2 pg 3, we prove that the origin **is S, not AS**\n",
    "\n",
    "(ii) Given initial conditions $(\\omega_{10},\\omega_{20},\\omega_{30})^{\\top}$ and parameters $J_1 \\neq J_2 \\neq J_3$, it is possible to explicitly solve for the flow (still assuming $\\tau_1 = \\tau_2 = \\tau_3 = 0$) as\n",
    "\\begin{align*}\n",
    "\\omega_1(t) = \\overline{\\omega}_{10} \\mathrm{cn}\\left(\\omega_{p}t + \\varepsilon, m\\right),\\\\\n",
    "\\omega_2(t) = \\overline{\\omega}_{20} \\mathrm{sn}\\left(\\omega_{p}t + \\varepsilon, m\\right),\\\\\n",
    "\\omega_3(t) = \\overline{\\omega}_{30} \\mathrm{dn}\\left(\\omega_{p}t + \\varepsilon, m\\right),\n",
    "\\end{align*}\n",
    "where $\\overline{\\omega}_{10},\\overline{\\omega}_{20},\\overline{\\omega}_{30},\\omega_{p},\\varepsilon,m$ depend only on $(\\omega_{10},\\omega_{20},\\omega_{30})^{\\top}$ and $J_1,J_2,J_3$. The functions $\\mathrm{cn},\\mathrm{sn},\\mathrm{dn}$ are the so-called Jacobi elliptic functions and are periodic in time $t$. **Using this information alone, and ignoring the previous Lyapunov analysis, explain what can you conclude** about the asymptotic stability of the origin?\n",
    "\n",
    "1. If the $\\omega_{i}(t)$ terms are **periodic** then by definition they by definition they do **not** converge to any one value i.e. at some starting time and period $t_{1}, p_{1}$, $\\omega_{i}(t_{1}) = \\omega_{i}(t_{1} + k_{1}p_{1}) = \\alpha$ for $k_{1} = 1, 2, 3, ... \\infty$ and for some other $t_{2}, p_{2}$, $\\omega_{i}(t_{2}) = \\omega_{i}(t_{2} + k_{2}p_{2}) = \\beta$ for $k_{2} = 1, 2, 3, ... \\infty$ s.t. $\\alpha \\neq \\beta$\n",
    "<br>\n",
    "2. So if $\\omega_{i}(t)$ converges, then that means $\\lim_{t \\to +\\infty} w_{i}(t) = w_{i}(t_{1} + k_{1}p_{1}) = w_{i}(t_{2} + k_{2}p_{2}) = \\gamma$ but this contradicts the statement in 1. So $\\omega_{i}(t)$ **does not converge**\n",
    "<br>\n",
    "3. Thus by definition, given $\\omega_{i}(t)$ the origin is **not AS**"
   ]
  },
  {
   "cell_type": "markdown",
   "metadata": {},
   "source": [
    "## (c) [25 points] Global asymptotic stabilization using feedback control\n",
    "\n",
    "For $i=1,2,3$, consider the state feedback control law $\\tau_i = -k_i\\omega_i$, where $k_i>0$ are constants. **Prove that** origin of the closed-loop system is globally asymptotically stable (GAS).\n",
    "\n",
    "1. Let $V = \\frac{1}{2}\\begin{bmatrix} \\omega_{1} & \\omega_{2} & \\omega_{3} \\end{bmatrix} \\begin{bmatrix} J_{1} & 0 & 0 \\\\ 0 & J_{2} & 0 \\\\ 0 & 0 & J_{3} \\end{bmatrix} \\begin{bmatrix} \\omega_{1} \\\\ \\omega_{2} \\\\ \\omega_{3} \\end{bmatrix} = \\frac{1}{2}(J_{1}\\omega_{1}^{2} + J_{2}\\omega_{2}^{2} + J_{3}\\omega_{3}^{2})$ where $P = \\begin{bmatrix} J_{1} & 0 & 0 \\\\ 0 & J_{2} & 0 \\\\ 0 & 0 & J_{3} \\end{bmatrix}$\n",
    "<br>\n",
    "2. Knowing $J_{1}, J_{2}, J_{3} > 0$, $V = \\frac{1}{2}(J_{1}\\omega_{1}^{2} + J_{2}\\omega_{2}^{2} + J_{3}\\omega_{3}^{2}) > 0$ $\\forall \\begin{bmatrix} \\omega_{1} & \\omega_{2} & \\omega_{3} \\end{bmatrix} \\rightarrow$ P is positive definite matrix.\n",
    "<br>\n",
    "3. We can also see that since all terms in V are non-negative, $\\lim_{\\lVert w \\rVert \\to +\\infty} V = +\\infty$ so by definition V is radially unbounded.\n",
    "<br>\n",
    "4. We can show that $\\dot{V}$ is negative definite:\n",
    "\\begin{align}\n",
    "& \\dot{V} = \\omega_{1}(J_{1}*\\dot\\omega_{1}) + \\omega_{2}(J_{2}*\\dot\\omega_{2}) + \\omega_{3}(J_{3}*\\dot\\omega_{3}) \\\\\n",
    "& = \\omega_{1}(J_{2}-J_{3})\\omega_{2}\\omega_{3} - k_{1}\\omega_{1}^{2} + \\omega_{2}(J_{3}-J_{1})\\omega_{1}\\omega_{3} - k_{2}\\omega_{2}^{2} + \\omega_{3}(J_{1}-J_{2})\\omega_{1}\\omega_{1} - k_{3}\\omega_{3}^{2} \\\\\n",
    "& = \\omega_{1}\\omega_{2}\\omega_{3}(J_{2}-J_{3} + J_{3}-J_{1} + J_{1}-J_{2}) - k_{1}\\omega_{1}^{2} - k_{2}\\omega_{2}^{2} - k_{3}\\omega_{3}^{2} \\\\\n",
    "& = \\omega_{1}\\omega_{2}\\omega_{3}(J_{2}-J_{3} + J_{3}-J_{1} + J_{1}-J_{2}) - k_{1}\\omega_{1}^{2} - k_{2}\\omega_{2}^{2} - k_{3}\\omega_{3}^{2} \\\\\n",
    "& = 0 - k_{1}\\omega_{1}^{2} - k_{2}\\omega_{2}^{2} - k_{3}\\omega_{3}^{2} \\\\\n",
    "& = - (k_{1}\\omega_{1}^{2} + k_{2}\\omega_{2}^{2} + k_{3}\\omega_{3}^{2}) < 0 \\\\\n",
    "\\end{align}\n",
    "<br>\n",
    "5. From 2., 3. 4., and by Lecture 3 pg 9, we prove that **the origin is GAS**"
   ]
  }
 ],
 "metadata": {
  "kernelspec": {
   "display_name": "Python 3 (ipykernel)",
   "language": "python",
   "name": "python3"
  },
  "language_info": {
   "codemirror_mode": {
    "name": "ipython",
    "version": 3
   },
   "file_extension": ".py",
   "mimetype": "text/x-python",
   "name": "python",
   "nbconvert_exporter": "python",
   "pygments_lexer": "ipython3",
   "version": "3.8.10"
  }
 },
 "nbformat": 4,
 "nbformat_minor": 4
}
